introduce new definition to capture the propagation of Boogie commands that preserve a Viper-to-Boogie state relation
the reason for using a definition is the hope is that one can better control the state relation instantations while propagating Boogie commands (before the lack of control led to the generated proofs failing in certain cases due to an incorrect instantiation)

BoogieInterface.thy
@@ -1,5 +1,5 @@
 theory BoogieInterface
-imports Boogie_Lang.Ast
+imports Boogie_Lang.Ast TotalUtil
 begin
 
 subsection \<open>Expressions\<close>
@@ -126,6 +126,36 @@ lemma red_ast_bpl_if_nondet_else:
   by simp
 
 subsection \<open>Reducing Boogie programs while preserving a property\<close>
+
+subsection \<open>red_ast_bpl_rel\<close>
+
+definition red_ast_bpl_rel 
+  where "red_ast_bpl_rel R0 R1 P ctxt \<gamma>0 \<gamma>1 \<equiv>
+          \<forall> \<omega> ns. R0 \<omega> ns \<longrightarrow> (\<exists>ns'. red_ast_bpl P ctxt (\<gamma>0, Normal ns) (\<gamma>1, Normal ns') \<and> R1 \<omega> ns')"
+
+lemma red_ast_bpl_rel_reflexive:
+  shows "red_ast_bpl_rel R R P ctxt \<gamma> \<gamma>"  
+  using red_ast_bpl_refl
+  unfolding red_ast_bpl_rel_def
+  by blast  
+
+lemma red_ast_bpl_rel_transitive:
+  assumes "red_ast_bpl_rel R0 R1 P ctxt \<gamma>0 \<gamma>1"
+      and "red_ast_bpl_rel R1 R2 P ctxt \<gamma>1 \<gamma>2"
+    shows "red_ast_bpl_rel R0 R2 P ctxt \<gamma>0 \<gamma>2"
+  using assms red_ast_bpl_transitive
+  unfolding red_ast_bpl_rel_def
+  by blast
+
+lemma red_ast_bpl_rel_one_simple_cmd:
+  assumes "\<And> \<omega> ns. R0 \<omega> ns \<Longrightarrow>
+                \<exists>ns'. ( (type_interp ctxt), ([] :: ast proc_context), (var_context ctxt), (fun_interp ctxt), rtype_interp ctxt \<turnstile> \<langle>c, Normal ns\<rangle> \<rightarrow> (Normal ns')) \<and>
+                R1 \<omega> ns'"
+  shows "red_ast_bpl_rel R0 R1 P ctxt (BigBlock name (c#cs) str tr, cont) (BigBlock name cs str tr, cont)"
+  using assms
+  unfolding red_ast_bpl_rel_def red_ast_bpl_def
+  by blast
+
 
 lemma red_ast_bpl_propagate_rel:
   assumes "red_ast_bpl P ctxt (\<gamma>0, Normal ns0) (\<gamma>1, Normal ns1)" and
